Add an initial glue file in the pipeline, no option in bounds
We can do bounds analysis without options.

Also, add some tactics from another branch for the glue to start the
reflective pipeline.

src/Reflection/Z/Bounds/Interpretation.v
@@ -2,7 +2,6 @@ Require Import Coq.ZArith.ZArith.
 Require Import Crypto.Reflection.Z.Syntax.
 Require Import Crypto.Reflection.Syntax.
 Require Import Crypto.Reflection.Relations.
-Require Import Crypto.Util.Option.
 Require Import Crypto.Util.Notations.
 Require Import Crypto.Util.Decidable.
 Require Import Crypto.Util.ZRange.
@@ -15,73 +14,70 @@ Local Notation eta4 x := (eta3 (fst x), snd x).
 
 Notation bounds := zrange.
 Delimit Scope bounds_scope with bounds.
+Local Open Scope Z_scope.
 
 Module Import Bounds.
-  Definition t := option bounds. (* TODO?: Separate out the bounds computation from the overflow computation? e.g., have [safety := in_bounds | overflow] and [t := bounds * safety]? *)
+  Definition t := bounds.
   Bind Scope bounds_scope with t.
   Local Coercion Z.of_nat : nat >-> Z.
   Section with_bitwidth.
     Context (bit_width : option Z).
-    Definition SmartBuildBounds (l u : Z)
-      := if ((0 <=? l) && (match bit_width with Some bit_width => u <? 2^bit_width | None => true end))%Z%bool
-         then Some {| lower := l ; upper := u |}
-         else None.
-    Definition SmartRebuildBounds (b : t) : t
-      := match b with
-         | Some b => SmartBuildBounds (lower b) (upper b)
-         | None => None
+    Definition four_corners (f : Z -> Z -> Z) : t -> t -> t
+      := fun x y
+         => let (lx, ux) := x in
+            let (ly, uy) := y in
+            {| lower := Z.min (f lx ly) (Z.min (f lx uy) (Z.min (f ux ly) (f ux uy)));
+               upper := Z.max (f lx ly) (Z.max (f lx uy) (Z.max (f ux ly) (f ux uy))) |}.
+    Definition truncation_bounds (b : t)
+      := match bit_width with
+         | Some bit_width => if ((0 <=? lower b) && (upper b <? 2^bit_width))%bool
+                             then b
+                             else {| lower := 0 ; upper := 2^bit_width - 1 |}
+         | None => b
          end.
+    Definition BuildTruncated_bounds (l u : Z) : t
+      := truncation_bounds {| lower := l ; upper := u |}.
     Definition t_map1 (f : bounds -> bounds) (x : t)
-      := match x with
-         | Some x
-           => match f x with
-              | {| lower := l ; upper := u |}
-                => SmartBuildBounds l u
-              end
-         | _ => None
-         end%Z.
-    Definition t_map2 (f : bounds -> bounds -> bounds) (x y : t)
-      := match x, y with
-         | Some x, Some y
-           => match f x y with
-              | {| lower := l ; upper := u |}
-                => SmartBuildBounds l u
-              end
-         | _, _ => None
-         end%Z.
+      := truncation_bounds (f x).
+    Definition t_map2 (f : Z -> Z -> Z) : t -> t -> t
+      := fun x y => truncation_bounds (four_corners f x y).
     Definition t_map4 (f : bounds -> bounds -> bounds -> bounds -> bounds) (x y z w : t)
-      := match x, y, z, w with
-         | Some x, Some y, Some z, Some w
-           => match f x y z w with
-              | {| lower := l ; upper := u |}
-                => SmartBuildBounds l u
-              end
-         | _, _, _, _ => None
-         end%Z.
-    Definition add' : bounds -> bounds -> bounds
-      := fun x y => let (lx, ux) := x in let (ly, uy) := y in {| lower := lx + ly ; upper := ux + uy |}.
-    Definition add : t -> t -> t := t_map2 add'.
-    Definition sub' : bounds -> bounds -> bounds
-      := fun x y => let (lx, ux) := x in let (ly, uy) := y in {| lower := lx - uy ; upper := ux - ly |}.
-    Definition sub : t -> t -> t := t_map2 sub'.
-    Definition mul' : bounds -> bounds -> bounds
-      := fun x y => let (lx, ux) := x in let (ly, uy) := y in {| lower := lx * ly ; upper := ux * uy |}.
-    Definition mul : t -> t -> t := t_map2 mul'.
-    Definition shl' : bounds -> bounds -> bounds
-      := fun x y => let (lx, ux) := x in let (ly, uy) := y in {| lower := Z.shiftl lx ly ; upper := Z.shiftl ux uy |}.
-    Definition shl : t -> t -> t := t_map2 shl'.
-    Definition shr' : bounds -> bounds -> bounds
-      := fun x y => let (lx, ux) := x in let (ly, uy) := y in {| lower := Z.shiftr lx uy ; upper := Z.shiftr ux ly |}.
-    Definition shr : t -> t -> t := t_map2 shr'.
-    Definition land' : bounds -> bounds -> bounds
-      := fun x y => let (lx, ux) := x in let (ly, uy) := y in {| lower := 0 ; upper := Z.min ux uy |}.
-    Definition land : t -> t -> t := t_map2 land'.
-    Definition lor' : bounds -> bounds -> bounds
-      := fun x y => let (lx, ux) := x in let (ly, uy) := y in
-                                         {| lower := Z.max lx ly;
-                                            upper := 2^(Z.max (Z.log2_up (ux+1)) (Z.log2_up (uy+1))) - 1 |}.
-    Definition lor : t -> t -> t := t_map2 lor'.
-    Definition neg' (int_width : Z) : bounds -> bounds
+      := truncation_bounds (f x y z w).
+    Definition add : t -> t -> t := t_map2 Z.add.
+    Definition sub : t -> t -> t := t_map2 Z.sub.
+    Definition mul : t -> t -> t := t_map2 Z.mul.
+    Definition shl : t -> t -> t := t_map2 Z.shiftl.
+    Definition shr : t -> t -> t := t_map2 Z.shiftr.
+    Definition extreme_lor_land_bounds (x y : t) : t
+      := let (lx, ux) := x in
+         let (ly, uy) := y in
+         let lx := Z.abs lx in
+         let ly := Z.abs ly in
+         let ux := Z.abs ux in
+         let uy := Z.abs uy in
+         let max := Z.max (Z.max lx ly) (Z.max ux uy) in
+         {| lower := -2^(1 + Z.log2_up max) ; upper := 2^(1 + Z.log2_up max) |}.
+    Definition extermization_bounds (f : t -> t -> t) (x y : t) : t
+      := truncation_bounds
+           (let (lx, ux) := x in
+            let (ly, uy) := y in
+            if ((lx <? 0) || (ly <? 0))%Z%bool
+            then extreme_lor_land_bounds x y
+            else f x y).
+    Definition land : t -> t -> t
+      := extermization_bounds
+           (fun x y
+            => let (lx, ux) := x in
+               let (ly, uy) := y in
+               {| lower := Z.min 0 (Z.min lx ly) ; upper := Z.max 0 (Z.min ux uy) |}).
+    Definition lor : t -> t -> t
+      := extermization_bounds
+           (fun x y
+            => let (lx, ux) := x in
+               let (ly, uy) := y in
+               {| lower := Z.max lx ly;
+                  upper := 2^(Z.max (Z.log2_up (ux+1)) (Z.log2_up (uy+1))) - 1 |}).
+    Definition neg' (int_width : Z) : t -> t
       := fun v
          => let (lb, ub) := v in
             let might_be_one := ((lb <=? 1) && (1 <=? ub))%Z%bool in
@@ -89,19 +85,23 @@ Module Import Bounds.
             if must_be_one
             then {| lower := Z.ones int_width ; upper := Z.ones int_width |}
             else if might_be_one
-                 then {| lower := 0 ; upper := Z.ones int_width |}
+                 then {| lower := Z.min 0 (Z.ones int_width) ; upper := Z.max 0 (Z.ones int_width) |}
                  else {| lower := 0 ; upper := 0 |}.
     Definition neg (int_width : Z) : t -> t
       := fun v
-         => if ((0 <=? int_width) (*&& (int_width <=? WordW.bit_width)*))%Z%bool
-            then t_map1 (neg' int_width) v
-            else None.
-    Definition cmovne' (r1 r2 : bounds) : bounds
-      := let (lr1, ur1) := r1 in let (lr2, ur2) := r2 in {| lower := Z.min lr1 lr2 ; upper := Z.max ur1 ur2 |}.
-    Definition cmovne (x y r1 r2 : t) : t := t_map4 (fun _ _ => cmovne') x y r1 r2.
-    Definition cmovle' (r1 r2 : bounds) : bounds
-      := let (lr1, ur1) := r1 in let (lr2, ur2) := r2 in {| lower := Z.min lr1 lr2 ; upper := Z.max ur1 ur2 |}.
-    Definition cmovle (x y r1 r2 : t) : t := t_map4 (fun _ _ => cmovle') x y r1 r2.
+         => truncation_bounds (neg' int_width v).
+    Definition cmovne' (r1 r2 : t) : t
+      := let (lr1, ur1) := r1 in
+         let (lr2, ur2) := r2 in
+         {| lower := Z.min lr1 lr2 ; upper := Z.max ur1 ur2 |}.
+    Definition cmovne (x y r1 r2 : t) : t
+      := truncation_bounds (cmovne' r1 r2).
+    Definition cmovle' (r1 r2 : t) : t
+      := let (lr1, ur1) := r1 in
+         let (lr2, ur2) := r2 in
+         {| lower := Z.min lr1 lr2 ; upper := Z.max ur1 ur2 |}.
+    Definition cmovle (x y r1 r2 : t) : t
+      := truncation_bounds (cmovle' r1 r2).
   End with_bitwidth.
 
   Module Export Notations.
@@ -124,8 +124,8 @@ Module Import Bounds.
 
   Definition interp_op {src dst} (f : op src dst) : interp_flat_type interp_base_type src -> interp_flat_type interp_base_type dst
     := match f in op src dst return interp_flat_type interp_base_type src -> interp_flat_type interp_base_type dst with
-       | OpConst TZ v => fun _ => SmartBuildBounds None v v
-       | OpConst (TWord _ as T) v => fun _ => SmartBuildBounds (bit_width_of_base_type T) ((*FixedWordSizes.wordToZ*) v) ((*FixedWordSizes.wordToZ*) v)
+       | OpConst TZ v => fun _ => BuildTruncated_bounds None v v
+       | OpConst (TWord _ as T) v => fun _ => BuildTruncated_bounds (bit_width_of_base_type T) ((*FixedWordSizes.wordToZ*) v) ((*FixedWordSizes.wordToZ*) v)
        | Add T => fun xy => add (bit_width_of_base_type T) (fst xy) (snd xy)
        | Sub T => fun xy => sub (bit_width_of_base_type T) (fst xy) (snd xy)
        | Mul T => fun xy => mul (bit_width_of_base_type T) (fst xy) (snd xy)
@@ -136,63 +136,29 @@ Module Import Bounds.
        | Neg T int_width => fun x => neg (bit_width_of_base_type T) int_width x
        | Cmovne T => fun xyzw => let '(x, y, z, w) := eta4 xyzw in cmovne (bit_width_of_base_type T) x y z w
        | Cmovle T => fun xyzw => let '(x, y, z, w) := eta4 xyzw in cmovle (bit_width_of_base_type T) x y z w
-       | Cast _ T => fun x => SmartRebuildBounds (bit_width_of_base_type T) x
+       | Cast _ T => fun x => truncation_bounds (bit_width_of_base_type T) x
        end%bounds.
 
-  Definition of_Z (z : Z) : t := Some (ZToZRange z).
+  Definition of_Z (z : Z) : t := ZToZRange z.
 
   Definition of_interp t (z : Syntax.interp_base_type t) : interp_base_type t
-    := Some (ZToZRange (match t return Syntax.interp_base_type t -> Z with
-                        | TZ => fun z => z
-                        | TWord logsz => fun z => z (*FixedWordSizes.wordToZ*)
-                        end z)).
+    := ZToZRange (interpToZ z).
 
-  Definition bounds_to_base_type' (b : bounds) : base_type
+  Definition bounds_to_base_type (b : t) : base_type
     := if (0 <=? lower b)%Z
        then TWord (Z.to_nat (Z.log2_up (Z.log2_up (1 + upper b))))
        else TZ.
-  Definition bounds_to_base_type (b : t) : base_type
-    := match b with
-       | None => TZ
-       | Some b' => bounds_to_base_type' b'
-       end.
 
   Definition ComputeBounds {t} (e : Expr base_type op t)
              (input_bounds : interp_flat_type interp_base_type (domain t))
     : interp_flat_type interp_base_type (codomain t)
     := Interp (@interp_op) e input_bounds.
 
-  Definition bound_is_goodb : forall t, interp_base_type t -> bool
-    := fun t bs
-       => match bs with
-          | Some bs
-            => (*let l := lower bs in
-               let u := upper bs in
-               let bit_width := bit_width_of_base_type t in
-               ((0 <=? l) && (match bit_width with Some bit_width => Z.log2 u <? bit_width | None => true end))%Z%bool*)
-            true
-          | None => false
-          end.
-  Definition bound_is_good : forall t, interp_base_type t -> Prop
-    := fun t v => bound_is_goodb t v = true.
-  Definition bounds_are_good : forall {t}, interp_flat_type interp_base_type t -> Prop
-    := (@interp_flat_type_rel_pointwise1 _ _ bound_is_good).
-
   Definition is_tighter_thanb' {T} : interp_base_type T -> interp_base_type T -> bool
-    := fun bounds1 bounds2
-       => match bounds1, bounds2 with
-          | Some bounds1, Some bounds2 => is_tighter_than_bool bounds1 bounds2
-          | _, None => true
-          | None, Some _ => false
-          end.
+    := is_tighter_than_bool.
 
   Definition is_bounded_by' {T} : interp_base_type T -> Syntax.interp_base_type T -> Prop
-    := fun bounds val
-       => match bounds with
-          | Some bounds'
-            => is_bounded_by' (bit_width_of_base_type T) bounds' val
-          | None => True
-          end.
+    := fun bounds val => is_bounded_by' (bit_width_of_base_type T) bounds (interpToZ val).
 
   Definition is_tighter_thanb {T} : interp_flat_type interp_base_type T -> interp_flat_type interp_base_type T -> bool
     := interp_flat_type_relb_pointwise (@is_tighter_thanb').
