src/Reflection/Z/Bounds/Pipeline/Glue.v
@@ -1,0 +1,149 @@
+(** * Reflective Pipeline: Glue Code *)
+(** This file defines the tactics that transform a non-reflective goal
+    into a goal the that the reflective machinery can handle. *)
+Require Import Crypto.Reflection.Syntax.
+Require Import Crypto.Reflection.Reify.
+Require Import Crypto.Reflection.Z.Syntax.
+Require Import Crypto.Reflection.Z.Syntax.Util.
+Require Import Crypto.Reflection.Z.Reify.
+Require Import Crypto.Reflection.Z.Bounds.Interpretation.
+Require Import Crypto.Util.Tactics.Head.
+Require Import Crypto.Util.Curry.
+Require Import Crypto.Util.FixedWordSizes.
+Require Import Crypto.Util.BoundedWord.
+Require Import Crypto.Util.Tuple.
+
+(** The [do_curry] tactic takes a goal of the form
+<<
+BoundedWordToZ (?f a b ... z) = F A B ... Z
+>>
+    and turns it into a goal of the form
+<<
+BoundedWordToZ (f' (a, b, ..., z)) = F' (A, B, ..., Z)
+>>
+ *)
+Ltac do_curry :=
+  lazymatch goal with
+  | [ |- ?BWtoZ ?f_bw = ?f_Z ]
+    => let f_bw := head f_bw in
+       let f_Z := head f_Z in
+       change_with_curried f_Z;
+       let f_bw_name := fresh f_bw in
+       set (f_bw_name := f_bw);
+       change_with_curried f_bw_name
+  end.
+(** The [split_BoundedWordToZ] tactic takes a goal of the form
+<<
+BoundedWordToZ (f args) = F ARGS
+>>
+    and splits it into a conjunction, one part about the computational
+    behavior, and another part about the boundedness.  *)
+Ltac count_tuple_length T :=
+  lazymatch T with
+  | (?A * ?B)%type => let a := count_tuple_length A in
+                      let b := count_tuple_length B in
+                      (eval compute in (a + b)%nat)
+  | _ => constr:(1%nat)
+  end.
+Ltac make_evar_for_first_projection :=
+  lazymatch goal with
+  | [ |- @map ?N1 ?A ?B wordToZ (@proj1_sig _ ?P ?f) = ?fZ ?argsZ ]
+    => let T := type of argsZ in
+       let N := count_tuple_length T in
+       let map' := (eval compute in (@map N)) in
+       let proj1_sig' := (eval compute in @proj1_sig) in
+       let f1 := fresh f in
+       let f2 := fresh f in
+       let pf := fresh in
+       revert f; refine (_ : let f := exist P _ _ in _);
+       intro f;
+       pose (proj1_sig f) as f1;
+       pose (proj2_sig f : P f1) as f2;
+       change f with (exist _ f1 f2);
+       subst f; cbn [proj1_sig proj2_sig] in f1, f2 |- *; revert f2;
+       lazymatch goal with
+       | [ |- let f' := _ in @?P f' ]
+         => refine (let pf := _ in (proj2 pf : let f' := proj1 pf in P f'))
+       end
+  end.
+Ltac split_BoundedWordToZ :=
+  match goal with
+  | [ |- BoundedWordToZ _ _ _ ?x = _ ]
+    => revert x
+  end;
+  repeat match goal with
+         | [ |- context[BoundedWordToZ _ _ _ ?x] ]
+           => is_var x;
+              first [ clearbody x; fail 1
+                    | instantiate (1:=ltac:(destruct x)); destruct x ]
+         end;
+  cbv beta iota; intro;
+  unfold BoundedWordToZ; cbn [proj1_sig];
+  make_evar_for_first_projection.
+(** The [zrange_to_reflective] tactic takes a goal of the form
+<<
+is_bounded_by _ bounds (map wordToZ (?fW args)) /\ map wordToZ (?fW args) = fZ argsZ
+>>
+    and uses [cut] and a small lemma to turn it into a goal that the
+    reflective machinery can handle.  The goal left by this tactic
+    should be fully solvable by the reflective pipeline. *)
+
+Ltac const_tuple T val :=
+  lazymatch T with
+  | (?A * ?B)%type => let a := const_tuple A val in
+                      let b := const_tuple B val in
+                      constr:((a, b)%core)
+  | _ => val
+  end.
+Lemma adjust_goal_for_reflective {T P} (LHS RHS : T)
+  : P RHS /\ LHS = RHS -> P LHS /\ LHS = RHS.
+Proof. intros [? ?]; subst; tauto. Qed.
+Ltac adjust_goal_for_reflective := apply adjust_goal_for_reflective.
+Ltac unmap_wordToZ_tuple term :=
+  lazymatch term with
+  | (?x, ?y) => let x' := unmap_wordToZ_tuple x in
+                let y' := unmap_wordToZ_tuple y in
+                constr:((x', y'))
+  | map wordToZ ?x => x
+  end.
+Ltac zrange_to_reflective_hyps_step :=
+  match goal with
+  | [ H : @ZRange.is_bounded_by ?option_bit_width ?count ?bounds (Tuple.map wordToZ ?arg) |- _ ]
+    => let rT := constr:(Syntax.tuple (Tbase TZ) count) in
+       let is_bounded_by' := constr:(@Bounds.is_bounded_by rT) in
+       let map' := constr:(@cast_back_flat_const (@Bounds.interp_base_type) rT (fun _ => Bounds.bounds_to_base_type) bounds) in
+       (* we use [cut] and [abstract] rather than [change] to catch inefficiencies in conversion early, rather than allowing [Defined] to take forever *)
+       let H' := fresh H in
+       rename H into H';
+       assert (H : is_bounded_by' bounds (map' arg)) by (clear -H'; abstract exact H');
+       clear H'; move H at top
+  end.
+Ltac zrange_to_reflective_hyps := repeat zrange_to_reflective_hyps_step.
+Ltac zrange_to_reflective_goal :=
+  lazymatch goal with
+  | [ |- @ZRange.is_bounded_by ?option_bit_width ?count ?bounds (Tuple.map wordToZ ?reified_f_evar)
+         /\ Tuple.map wordToZ ?reified_f_evar = ?f ?Zargs ]
+    => let T := type of f in
+       let f_domain := lazymatch T with ?A -> ?B => A end in
+       let T := (eval compute in T) in
+       let rT := reify_type T in
+       let is_bounded_by' := constr:(@Bounds.is_bounded_by (codomain rT)) in
+       let input_bounds := const_tuple f_domain bounds in
+       let map_t := constr:(fun t bs => @cast_back_flat_const (@Bounds.interp_base_type) t (fun _ => Bounds.bounds_to_base_type) bs) in
+       let map_output := constr:(map_t (codomain rT) bounds) in
+       let map_input := constr:(map_t (domain rT) input_bounds) in
+       let args := unmap_wordToZ_tuple Zargs in
+       (* we use [cut] and [abstract] rather than [change] to catch inefficiencies in conversion early, rather than allowing [Defined] to take forever *)
+       cut (is_bounded_by' bounds (map_output reified_f_evar) /\ map_output reified_f_evar = f (map_input args));
+       [ generalize reified_f_evar; clear; clearbody f; let x := fresh in intros ? x; abstract exact x
+       | ];
+       cbv beta
+  end;
+  adjust_goal_for_reflective.
+Ltac zrange_to_reflective := zrange_to_reflective_hyps; zrange_to_reflective_goal.
+
+(** The tactic [refine_to_reflective_glue] is the public-facing one. *)
+Ltac refine_to_reflective_glue :=
+  do_curry;
+  split_BoundedWordToZ;
+  zrange_to_reflective.
